Examples/IMP/Abstraction/Lemmas.lean
@@ -4,20 +4,12 @@ import Examples.IMP.Abstraction.Defs
 
 namespace Examples.IMP
 
-@[simp] theorem controlOfConfig_running (s : Stmt) (σ : Store) :
-    controlOfConfig (.running s σ) = .running s :=
+@[simp] theorem controlOfConfig_mk (s : Stmt) (σ : Store) :
+    controlOfConfig (s, σ) = s :=
   rfl
 
-@[simp] theorem controlOfConfig_done (σ : Store) :
-    controlOfConfig (.done σ) = .done :=
-  rfl
-
-@[simp] theorem storeOfConfig_running (s : Stmt) (σ : Store) :
-    storeOfConfig (.running s σ) = σ :=
-  rfl
-
-@[simp] theorem storeOfConfig_done (σ : Store) :
-    storeOfConfig (.done σ) = σ :=
+@[simp] theorem storeOfConfig_mk (s : Stmt) (σ : Store) :
+    storeOfConfig (s, σ) = σ :=
   rfl
 
 @[simp] theorem mem_gammaStoreOf
@@ -28,23 +20,14 @@ namespace Examples.IMP
     σ ∈ gammaStoreOf gamma ρ ↔ ∀ x : Var, σ x ∈ gamma (ρ x) :=
   Iff.rfl
 
-@[simp] theorem mem_gammaConfigOf_running
+@[simp] theorem mem_gammaConfigOf_mk
     {Abstract : Type _}
     {gamma : Abstract → Set Int}
     {κ : ConfigSharp Abstract}
     {s : Stmt}
     {σ : Store} :
-    (.running s σ) ∈ gammaConfigOf gamma κ ↔
-      σ ∈ gammaStoreOf gamma (κ (.running s)) :=
-  Iff.rfl
-
-@[simp] theorem mem_gammaConfigOf_done
-    {Abstract : Type _}
-    {gamma : Abstract → Set Int}
-    {κ : ConfigSharp Abstract}
-    {σ : Store} :
-    (.done σ) ∈ gammaConfigOf gamma κ ↔
-      σ ∈ gammaStoreOf gamma (κ .done) :=
+    (s, σ) ∈ gammaConfigOf gamma κ ↔
+      σ ∈ gammaStoreOf gamma (κ s) :=
   Iff.rfl
 
 end Examples.IMP
